\documentclass{article}

\usepackage{amsmath}

\begin{document}
    \begin{equation}
        E^2 = (pc)^2 + (mc^2)^2
    \end{equation}
    \begin{equation}
        \lambda = \frac{h}{p}
    \end{equation}
    \begin{equation}
        \lambda_{\text{max}} = \frac{b}{T}
    \end{equation}
    \begin{equation}
        R_T = \frac{2\pi^5k^4}{15c^2h^2} A T^4
    \end{equation}
    \begin{equation}
        V_0 = \frac{h\nu}{e} - \frac{w_0}{e}
    \end{equation}
    \begin{equation}
        \lambda' = \lambda + \frac{h}{m_ec}(1-\cos\theta)
    \end{equation}
    \begin{equation}
        -\frac{\hbar^2}{2m} \frac{\delta^2 \psi}{\delta x^2} + U(x)\psi(x) = E\psi(x)
    \end{equation}
    \begin{equation}
        E = \frac{h^2}{2mL^2}(n_x^2 + n_y^2 + \dots)
    \end{equation}
    \begin{equation}
        \langle f(x) \rangle = \int_{-\infty}^{\infty} \psi^* f(x) \psi dx
    \end{equation}
    \begin{equation}
        \langle Q \rangle = \int_{-\infty}^{\infty} \psi^* \hat Q \psi dx
    \end{equation}
    \begin{equation}
        \hat p = -i\hbar \frac{\delta}{\delta x}
    \end{equation}
    \begin{equation}
        \hat H = -\frac{\hbar^2}{2m} \frac{\delta^2}{\delta x^2} + U(x)
    \end{equation}
    \begin{equation}
        E_n = \left(\frac{1}{2} + n\right) \hbar \omega_0
    \end{equation}


\end{document}
